Abstract lock interface

heap_lang/lib/ticket_lock.v
@@ -4,6 +4,7 @@ From iris.program_logic Require Import auth.
 From iris.proofmode Require Import invariants.
 From iris.heap_lang Require Import proofmode notation.
 From iris.algebra Require Import gset.
+From iris.heap_lang.lib Require Import lock.
 Import uPred.
 
 Definition wait_loop: val :=
@@ -43,65 +44,70 @@ Instance subG_tlockΣ {Σ} : subG tlockΣ Σ → tlockG Σ.
 Proof. intros [? [?%subG_inG _]%subG_inv]%subG_inv. split; apply _. Qed.
 
 Section proof.
-Context `{!heapG Σ, !tlockG Σ} (N : namespace) (HN: heapN ⊥ N).
+  Context `{!heapG Σ, !tlockG Σ} (N : namespace).
 
-Definition tickets_inv (n: nat) (gs: gset_disjUR nat) : iProp Σ :=
-  (gs = GSet (seq_set 0 n))%I.
+  Definition tickets_inv (n: nat) (gs: gset_disjUR nat) : iProp Σ :=
+    (gs = GSet (seq_set 0 n))%I.
 
-Definition lock_inv (γ1 γ2: gname) (lo ln: loc) (R : iProp Σ) : iProp Σ :=
-  (∃ (o n: nat),
+  Definition lock_inv (γ1 γ2: gname) (lo ln: loc) (R : iProp Σ) : iProp Σ :=
+    (∃ (o n: nat),
        lo ↦ #o ★ ln ↦ #n ★
        auth_inv γ1 (tickets_inv n) ★
        ((own γ2 (Excl ()) ★  R) ∨ auth_own γ1 (GSet {[ o ]})))%I.
 
-Definition is_lock (l: val) (R: iProp Σ) : iProp Σ :=
-  (∃ γ1 γ2 (lo ln: loc), heap_ctx ∧ l = (#lo, #ln)%V ∧ inv N (lock_inv γ1 γ2 lo ln R))%I.
+  Definition is_lock (γs: gname * gname) (l: val) (R: iProp Σ) : iProp Σ :=
+    (∃ (lo ln: loc),
+       heapN ⊥ N ∧ heap_ctx ∧
+       l = (#lo, #ln)%V ∧ inv N (lock_inv (fst γs) (snd γs) lo ln R))%I.
 
-Definition issued (l : val) (x: nat) (R : iProp Σ) : iProp Σ :=
-  (∃ γ1 γ2 (lo ln: loc), heap_ctx ∧ l = (#lo, #ln)%V ∧ inv N (lock_inv γ1 γ2 lo ln R) ∧
-                         auth_own γ1 (GSet {[ x ]}))%I.
+  Definition issued (γs: gname * gname) (l : val) (x: nat) (R : iProp Σ) : iProp Σ :=
+    (∃ (lo ln: loc),
+       heapN ⊥ N ∧ heap_ctx ∧
+       l = (#lo, #ln)%V ∧ inv N (lock_inv (fst γs) (snd γs) lo ln R) ∧
+       auth_own (fst γs) (GSet {[ x ]}))%I.
 
-Definition locked (l : val) (R : iProp Σ) : iProp Σ :=
-  (∃ γ1 γ2 (lo ln: loc), heap_ctx ∧ l = (#lo, #ln)%V ∧ inv N (lock_inv γ1 γ2 lo ln R) ∧
-                         own γ2 (Excl ()))%I.
+  Definition locked (γs: gname * gname) : iProp Σ := own (snd γs) (Excl ())%I.
 
-Global Instance lock_inv_ne n γ1 γ2 lo ln: Proper (dist n ==> dist n) (lock_inv γ1 γ2 lo ln).
-Proof. solve_proper. Qed.
-Global Instance is_lock_ne n l: Proper (dist n ==> dist n) (is_lock l).
-Proof. solve_proper. Qed.
-Global Instance locked_ne n l: Proper (dist n ==> dist n) (locked l).
-Proof. solve_proper. Qed.
+  Global Instance lock_inv_ne n γ1 γ2 lo ln : Proper (dist n ==> dist n) (lock_inv γ1 γ2 lo ln).
+  Proof. solve_proper. Qed.
+  Global Instance is_lock_ne γs n l : Proper (dist n ==> dist n) (is_lock γs l).
+  Proof. solve_proper. Qed.
+  Global Instance is_lock_persistent γs l R : PersistentP (is_lock γs l R).
+  Proof. apply _. Qed.
+  Global Instance locked_timeless γs : TimelessP (locked γs).
+  Proof. apply _. Qed.
 
-Global Instance is_lock_persistent l R : PersistentP (is_lock l R).
-Proof. apply _. Qed.
+  Lemma locked_exclusive (γs: gname * gname) : (locked γs ★ locked γs ⊢ False)%I.
+  Proof.
+    iIntros "[Hl Hl']". iCombine "Hl" "Hl'" as "Hl". by iDestruct (own_valid with "Hl") as %[].
+  Qed.
 
-Lemma newlock_spec (R : iProp Σ) Φ :
-  heap_ctx ★ R ★ (∀ l, is_lock l R -★ Φ l) ⊢ WP newlock #() {{ Φ }}.
+  Lemma newlock_spec (R : iProp Σ) Φ :
+    heapN ⊥ N → heap_ctx ★ R ★ (∀ lk γs, is_lock γs lk R -★ Φ lk) ⊢ WP newlock #() {{ Φ }}.
+  Proof.
+    iIntros (HN) "(#Hh & HR & HΦ)". rewrite /newlock.
+    wp_seq. wp_alloc lo as "Hlo". wp_alloc ln as "Hln".
+    iVs (own_alloc (Excl ())) as (γ2) "Hγ2"; first done.
+    iVs (own_alloc_strong (Auth (Excl' ∅) ∅) {[ γ2 ]}) as (γ1) "[% Hγ1]"; first done.
+    iVs (inv_alloc N _ (lock_inv γ1 γ2 lo ln R) with "[-HΦ]").
+    - iNext. rewrite /lock_inv.
+      iExists 0%nat, 0%nat.
+      iFrame.
+      iSplitL "Hγ1".
+      + rewrite /auth_inv.
+        iExists (GSet ∅).
+        by iFrame.
+      + iLeft. by iFrame.
+    - iVsIntro.
+      iSpecialize ("HΦ" $! (#lo, #ln)%V (γ1, γ2)). iApply "HΦ".
+      iExists lo, ln.
+      iSplit; by eauto.
+  Qed.
+
+Lemma wait_loop_spec γs l x R (Φ : val → iProp Σ) :
+  issued γs l x R ★ (locked γs -★ R -★ Φ #()) ⊢ WP wait_loop #x l {{ Φ }}.
 Proof.
-  iIntros "(#Hh & HR & HΦ)". rewrite /newlock /=.
-  wp_seq. wp_alloc lo as "Hlo". wp_alloc ln as "Hln".
-  iVs (own_alloc (Excl ())) as (γ2) "Hγ2"; first done.
-  iVs (own_alloc_strong (Auth (Excl' ∅) ∅) {[ γ2 ]}) as (γ1) "[% Hγ1]"; first done.
-  iVs (inv_alloc N _ (lock_inv γ1 γ2 lo ln R) with "[-HΦ]").
-  { iNext. rewrite /lock_inv.
-    iExists 0%nat, 0%nat.
-    iFrame.
-    iSplitL "Hγ1".
-    { rewrite /auth_inv.
-      iExists (GSet ∅).
-      by iFrame. }
-    iLeft.
-    by iFrame. }
-  iVsIntro.
-  iApply "HΦ".
-  iExists γ1, γ2, lo, ln.
-  iSplit; by auto.
-Qed.
-
-Lemma wait_loop_spec l x R (Φ : val → iProp Σ) :
-  issued l x R ★ (∀ l, locked l R -★ R -★ Φ #()) ⊢ WP wait_loop #x l {{ Φ }}.
-Proof.
-  iIntros "[Hl HΦ]". iDestruct "Hl" as (γ1 γ2 lo ln) "(#? & % & #? & Ht)".
+  iIntros "[Hl HΦ]". iDestruct "Hl" as (lo ln) "(% & #? & % & #? & Ht)".
   iLöb as "IH". wp_rec. subst. wp_let. wp_proj. wp_bind (! _)%E.
   iInv N as (o n) "[Hlo [Hln Ha]]" "Hclose".
   wp_load. destruct (decide (x = o)) as [->|Hneq].
@@ -110,7 +116,7 @@ Proof.
       { iNext. iExists o, n. iFrame. eauto. }
       iVsIntro. wp_let. wp_op=>[_|[]] //.
       wp_if. iVsIntro.
-      iApply ("HΦ" with "[-HR] HR"). iExists γ1, γ2, lo, ln; eauto.
+      iApply ("HΦ" with "[-HR] HR"). eauto.
     + iExFalso. iCombine "Ht" "Haown" as "Haown".
       iDestruct (auth_own_valid with "Haown") as % ?%gset_disj_valid_op.
       set_solver.
@@ -120,10 +126,10 @@ Proof.
     wp_if. iApply ("IH" with "Ht"). by iExact "HΦ".
 Qed.
 
-Lemma acquire_spec l R (Φ : val → iProp Σ) :
-  is_lock l R ★ (∀ l, locked l R -★ R -★ Φ #()) ⊢ WP acquire l {{ Φ }}.
+Lemma acquire_spec γs l R (Φ : val → iProp Σ) :
+  is_lock γs l R ★ (locked γs -★ R -★ Φ #()) ⊢ WP acquire l {{ Φ }}.
 Proof.
-  iIntros "[Hl HΦ]". iDestruct "Hl" as (γ1 γ2 lo ln) "(#? & % & #?)".
+  iIntros "[Hl HΦ]". iDestruct "Hl" as (lo ln) "(% & #? & % & #?)".
   iLöb as "IH". wp_rec. wp_bind (! _)%E. subst. wp_proj.
   iInv N as (o n) "[Hlo [Hln Ha]]" "Hclose".
   wp_load. iVs ("Hclose" with "[Hlo Hln Ha]").
@@ -145,8 +151,8 @@ Proof.
       rewrite Nat2Z.inj_succ -Z.add_1_r.
       iFrame. iExists (GSet (seq_set 0 (S n))). by iFrame. }
     iVsIntro. wp_if.
-    iApply (wait_loop_spec (#lo, #ln)).
-    iSplitR "HΦ"; last by done.
+    iApply (wait_loop_spec γs (#lo, #ln)).
+    iSplitR "HΦ"; last by auto.
     rewrite /issued /auth_own; eauto 10.
   - wp_cas_fail.
     iVs ("Hclose" with "[Hlo' Hln' Hainv Haown]").
@@ -154,10 +160,10 @@ Proof.
     iVsIntro. wp_if. by iApply "IH".
 Qed.
 
-Lemma release_spec R l (Φ : val → iProp Σ):
-  locked l R ★ R ★ Φ #() ⊢ WP release l {{ Φ }}.
+Lemma release_spec γs l R (Φ : val → iProp Σ):
+  is_lock γs l R ★ locked γs ★ R ★ Φ #() ⊢ WP release l {{ Φ }}.
 Proof.
-  iIntros "(Hl & HR & HΦ)"; iDestruct "Hl" as (γ1 γ2 lo ln) "(#? & % & #? & Hγ)".
+  iIntros "(Hl & Hγ & HR & HΦ)". iDestruct "Hl" as (lo ln) "(% & #? & % & #?)".
   iLöb as "IH". wp_rec. subst. wp_proj. wp_bind (! _)%E.
   iInv N as (o n) "[Hlo [Hln Hr]]" "Hclose".
   wp_load. iVs ("Hclose" with "[Hlo Hln Hr]").
@@ -182,3 +188,6 @@ Qed.
 End proof.
 
 Typeclasses Opaque is_lock issued locked.
+
+Definition ticket_lock `{!heapG Σ, !tlockG Σ} :=
+  Lock _ _ newlock acquire release (gname * gname) is_lock locked _ _ _ locked_exclusive newlock_spec acquire_spec release_spec.
